Abstract machine sem for delim_lang (cf biernack(a/i) danvy 2005)

theories/input_lang_delim/lang.v
@@ -23,31 +23,27 @@ Inductive expr {X : Set} :=
 (* The effects *)
 (* | Input : expr *)
 (* | Output (e : expr) : expr *)
-| Shift (e : expr) : expr
+| Shift (e : @expr (inc X)) : expr
 | Reset (e : expr) : expr
 with val {X : Set} :=
 | LitV (n : nat) : val
 | RecV (e : @expr (inc (inc X))) : val
-| ContV (e : @expr (inc X)) : val.
+| ContV (k : cont) : val
+with cont {X : Set} :=
+| END : cont
+| IfK (e1 : expr) (e2 : expr) : cont -> cont
+| AppLK (v : val) : cont -> cont (* ◻ v *)
+| AppRK (e : expr) : cont -> cont (* e ◻ *)
+| NatOpLK (op : nat_op) (v : val) : cont -> cont (* ◻ + v *)
+| NatOpRK (op : nat_op) (e : expr) : cont -> cont. (* e + ◻ *)
 
+(* conts are inside-out contexts: eg
+ IfK e1 e2 (AppLK v ◻) ==> App (if ◻ then e1 else e2) v*)
 
-
-Variant ectx_el {X : Set} :=
-  (* | OutputK : ectx_el *)
-  | IfK (e1 : @expr X) (e2 : @expr X) : ectx_el
-  | AppLK (v : @val X) : ectx_el (* ◻ v *)
-  | AppRK (e : @expr X) : ectx_el (* e ◻ *)
-  | NatOpLK (op : nat_op) (v : @val X) : ectx_el (* ◻ + v *)
-  | NatOpRK (op : nat_op) (e : @expr X) : ectx_el (* e + ◻ *)
-  | ResetK : ectx_el.
-
-
-Definition ectx {X : Set} := list (@ectx_el X).
 
 Arguments val X%bind : clear implicits.
 Arguments expr X%bind : clear implicits.
-Arguments ectx_el X%bind : clear implicits.
-Arguments ectx X%bind : clear implicits.
+Arguments cont X%bind : clear implicits.
 
 
 
@@ -64,7 +60,7 @@ Fixpoint emap {A B : Set} (f : A [→] B) (e : expr A) : expr B :=
   | If e₁ e₂ e₃ => If (emap f e₁) (emap f e₂) (emap f e₃)
   (* | Input => Input *)
   (* | Output e => Output (emap f e) *)
-  | Shift e => Shift (emap f e)
+  | Shift e => Shift (emap (f ↑) e)
   | Reset e => Reset (emap f e)
   end
 with
@@ -72,24 +68,22 @@ vmap {A B : Set} (f : A [→] B) (v : val A) : val B :=
   match v with
   | LitV n => LitV n
   | RecV e => RecV (emap ((f ↑) ↑) e)
-  | ContV e => ContV (emap (f ↑) e)
-  end.
+  | ContV k => ContV (kmap f k)
+  end
+with kmap {A B : Set} (f : A [→] B) (K : cont A) : cont B :=
+   match K with
+   | END => END
+   | IfK e1 e2 k => IfK (emap f e1) (emap f e2) (kmap f k)
+   | AppLK v k => AppLK (vmap f v) (kmap f k)
+   | AppRK e k => AppRK (emap f e) (kmap f k)
+   | NatOpLK op v k => NatOpLK op (vmap f v) (kmap f k)
+   | NatOpRK op e k => NatOpRK op (emap f e) (kmap f k)
+   end.
+
 
 #[export] Instance FMap_expr : FunctorCore expr := @emap.
 #[export] Instance FMap_val  : FunctorCore val := @vmap.
-
-Definition kmap {A B : Set} (f : A [→] B) (K : ectx A) : ectx B :=
-  map (fun x => match x with
-              (* | OutputK => OutputK *)
-              | IfK e1 e2 => IfK (fmap f e1) (fmap f e2)
-              | AppLK v => AppLK (fmap f v)
-              | AppRK e => AppRK (fmap f e)
-              | NatOpLK op v => NatOpLK op (fmap f v)
-              | NatOpRK op e => NatOpRK op (fmap f e)
-              | ResetK => ResetK
-              end) K.
-
-#[export] Instance FMap_ectx  : FunctorCore ectx := @kmap.
+#[export] Instance FMap_cont  : FunctorCore cont := @kmap.
 
 #[export] Instance SPC_expr : SetPureCore expr := @Var.
 
@@ -102,7 +96,7 @@ Fixpoint ebind {A B : Set} (f : A [⇒] B) (e : expr A) : expr B :=
   | If e₁ e₂ e₃ => If (ebind f e₁) (ebind f e₂) (ebind f e₃)
   (* | Input => Input *)
   (* | Output e => Output (ebind f e) *)
-  | Shift e => Shift (ebind f e)
+  | Shift e => Shift (ebind (f ↑) e)
   | Reset e => Reset (ebind f e)
   end
 with
@@ -110,36 +104,21 @@ vbind {A B : Set} (f : A [⇒] B) (v : val A) : val B :=
   match v with
   | LitV n => LitV n
   | RecV e => RecV (ebind ((f ↑) ↑) e)
-  | ContV e => ContV (ebind (f ↑) e)
-  end.
+  | ContV k => ContV (kbind f k)
+  end
+with kbind {A B : Set} (f : A [⇒] B) (K : cont A) : cont B :=
+   match K with
+   | END => END
+   | IfK e1 e2 k => IfK (ebind f e1) (ebind f e2) (kbind f k)
+   | AppLK v k => AppLK (vbind f v) (kbind f k)
+   | AppRK e k => AppRK (ebind f e) (kbind f k)
+   | NatOpLK op v k => NatOpLK op (vbind f v) (kbind f k)
+   | NatOpRK op e k => NatOpRK op (ebind f e) (kbind f k)
+   end.
 
 #[export] Instance BindCore_expr : BindCore expr := @ebind.
 #[export] Instance BindCore_val  : BindCore val := @vbind.
-
-Definition kbind {A B : Set} (f : A [⇒] B) (K : ectx A) : ectx B :=
-  map (fun x => match x with
-              (* | OutputK => OutputK *)
-              | IfK e1 e2 => IfK (bind f e1) (bind f e2)
-              | AppLK v => AppLK (bind f v)
-              | AppRK e => AppRK (bind f e)
-              | NatOpLK op v => NatOpLK op (bind f v)
-              | NatOpRK op e => NatOpRK op (bind f e)
-              | ResetK => ResetK
-              end) K.
-
-(* with kbind {A B : Set} (f : A [⇒] B) (K : ectx A) : ectx B := *)
-(*        match K with *)
-(*        | EmptyK => EmptyK *)
-(*        | OutputK K => OutputK (kbind f K) *)
-(*        | IfK K e₁ e₂ => IfK (kbind f K) (ebind f e₁) (ebind f e₂) *)
-(*        | AppLK K v => AppLK (kbind f K) (vbind f v) *)
-(*        | AppRK e K => AppRK (ebind f e) (kbind f K) *)
-(*        | NatOpRK op e K => NatOpRK op (ebind f e) (kbind f K) *)
-(*        | NatOpLK op K v => NatOpLK op (kbind f K) (vbind f v) *)
-(*        | ResetK K => ResetK (kbind f K) *)
-(*        end. *)
-
-#[export] Instance BindCore_ectx  : BindCore ectx := @kbind.
+#[export] Instance BindCore_cont  : BindCore cont := @kbind.
 
 #[export] Instance IP_typ : SetPure expr.
 Proof.
@@ -147,41 +126,25 @@ Proof.
 Qed.
 
 Fixpoint vmap_id X (δ : X [→] X) (v : val X) : δ ≡ ı → fmap δ v = v
-with emap_id X (δ : X [→] X) (e : expr X) : δ ≡ ı → fmap δ e = e.
-(* with kmap_id X (δ : X [→] X) (e : ectx X) : δ ≡ ı → fmap δ e = e. *)
+with emap_id X (δ : X [→] X) (e : expr X) : δ ≡ ı → fmap δ e = e
+with kmap_id X (δ : X [→] X) (k : cont X) : δ ≡ ı → fmap δ k = k.
 Proof.
   - auto_map_id.
   - auto_map_id.
+  - auto_map_id.
 Qed.
-
-Definition kmap_id X (δ : X [→] X) (k : ectx X) : δ ≡ ı -> fmap δ k = k.
-Proof.
-  rewrite  /fmap /FMap_ectx /kmap => H.
-  rewrite <-List.map_id. do 2 f_equal.
-  extensionality x. case: x => // >; rewrite !(emap_id, vmap_id)//.
-Qed.
-
 
 Fixpoint vmap_comp (A B C : Set) (f : B [→] C) (g : A [→] B) h (v : val A) :
   f ∘ g ≡ h → fmap f (fmap g v) = fmap h v
 with emap_comp (A B C : Set) (f : B [→] C) (g : A [→] B) h (e : expr A) :
+  f ∘ g ≡ h → fmap f (fmap g e) = fmap h e
+with kmap_comp (A B C : Set) (f : B [→] C) (g : A [→] B) h (e : cont A) :
   f ∘ g ≡ h → fmap f (fmap g e) = fmap h e.
 Proof.
   - auto_map_comp.
   - auto_map_comp.
+  - auto_map_comp.
 Qed.
-
-
-Definition kmap_comp (A B C : Set) (f : B [→] C) (g : A [→] B) h (e : ectx A) :
-  f ∘ g ≡ h → fmap f (fmap g e) = fmap h e.
-Proof.
-  rewrite  /fmap /FMap_ectx => H.
-  rewrite /kmap map_map. do 2 f_equal.
-  extensionality x.
-  case : x => // >; rewrite !(emap_comp _ _ _ f g h, vmap_comp _ _ _ f g h)//.
-Qed.
-
-
 
 #[export] Instance Functor_val : Functor val.
 Proof.
@@ -191,7 +154,7 @@ Qed.
 Proof.
   split; [exact emap_id | exact emap_comp].
 Qed.
-#[export] Instance Functor_ectx : Functor ectx.
+#[export] Instance Functor_cont : Functor cont.
 Proof.
   split; [exact kmap_id | exact kmap_comp].
 Qed.
@@ -199,6 +162,8 @@ Qed.
 Fixpoint vmap_vbind_pure (A B : Set) (f : A [→] B) (g : A [⇒] B) (v : val A) :
   f ̂ ≡ g → fmap f v = bind g v
 with emap_ebind_pure (A B : Set) (f : A [→] B) (g : A [⇒] B) (e : expr A) :
+  f ̂ ≡ g → fmap f e = bind g e
+with kmap_kbind_pure (A B : Set) (f : A [→] B) (g : A [⇒] B) (e : cont A) :
   f ̂ ≡ g → fmap f e = bind g e.
 Proof.
   - auto_map_bind_pure.
@@ -206,6 +171,7 @@ Proof.
     intros [| [| x]]; term_simpl; [reflexivity | reflexivity |].
     rewrite <-(EQ x).
     reflexivity.
+  - auto_map_bind_pure.
   - auto_map_bind_pure.
 Qed.
 
@@ -217,18 +183,7 @@ Qed.
 Proof.
   split; intros; now apply emap_ebind_pure.
 Qed.
-
-Definition kmap_kbind_pure (A B : Set) (f : A [→] B) (g : A [⇒] B) (e : ectx A) :
-  f ̂ ≡ g → fmap f e = bind g e.
-Proof.
-  rewrite /fmap /FMap_ectx /bind /BindCore_ectx /kmap /kbind => H.
-  do 2 f_equal. extensionality x.
-  case: x => [] > //; rewrite !(emap_ebind_pure _ _ _ g,
-                                  vmap_vbind_pure _ _ _ g)//.
-Qed.
-
-
-#[export] Instance BindMapPure_ectx : BindMapPure ectx.
+#[export] Instance BindMapPure_cont : BindMapPure cont.
 Proof.
   split; intros; now apply kmap_kbind_pure.
 Qed.
@@ -238,6 +193,9 @@ Fixpoint vmap_vbind_comm (A B₁ B₂ C : Set) (f₁ : B₁ [→] C) (f₂ : A [
   g₂ ∘ f₂ ̂ ≡ f₁ ̂ ∘ g₁ → bind g₂ (fmap f₂ v) = fmap f₁ (bind g₁ v)
 with emap_ebind_comm (A B₁ B₂ C : Set) (f₁ : B₁ [→] C) (f₂ : A [→] B₂)
        (g₁ : A [⇒] B₁) (g₂ : B₂ [⇒] C) (e : expr A) :
+  g₂ ∘ f₂ ̂ ≡ f₁ ̂ ∘ g₁ → bind g₂ (fmap f₂ e) = fmap f₁ (bind g₁ e)
+with kmap_kbind_comm (A B₁ B₂ C : Set) (f₁ : B₁ [→] C) (f₂ : A [→] B₂)
+       (g₁ : A [⇒] B₁) (g₂ : B₂ [⇒] C) (e : cont A) :
   g₂ ∘ f₂ ̂ ≡ f₁ ̂ ∘ g₁ → bind g₂ (fmap f₂ e) = fmap f₁ (bind g₁ e).
 Proof.
   - auto_map_bind_comm.
@@ -245,18 +203,8 @@ Proof.
     erewrite lift_comm; [reflexivity |].
     erewrite lift_comm; [reflexivity | assumption].
   - auto_map_bind_comm.
+  - auto_map_bind_comm.
 Qed.
-
-Definition kmap_kbind_comm (A B₁ B₂ C : Set) (f₁ : B₁ [→] C) (f₂ : A [→] B₂)
-       (g₁ : A [⇒] B₁) (g₂ : B₂ [⇒] C) (e : ectx A) :
-  g₂ ∘ f₂ ̂ ≡ f₁ ̂ ∘ g₁ → bind g₂ (fmap f₂ e) = fmap f₁ (bind g₁ e).
-Proof.
-  rewrite /fmap /FMap_ectx /bind /BindCore_ectx /kmap /kbind => H.
-  rewrite !map_map. do 2 f_equal. extensionality x.
-  case : x => // >; rewrite !(emap_ebind_comm _ B₁ _ _ f₁ _ g₁,
-                vmap_vbind_comm _ B₁ _ _ f₁ _ g₁)//.
-Qed.
-
 
 #[export] Instance BindMapComm_val : BindMapComm val.
 Proof.
@@ -266,7 +214,7 @@ Qed.
 Proof.
   split; intros; now apply emap_ebind_comm.
 Qed.
-#[export] Instance BindMapComm_ectx : BindMapComm ectx.
+#[export] Instance BindMapComm_cont : BindMapComm cont.
 Proof.
   split; intros; now apply kmap_kbind_comm.
 Qed.
@@ -274,27 +222,23 @@ Qed.
 Fixpoint vbind_id (A : Set) (f : A [⇒] A) (v : val A) :
   f ≡ ı → bind f v = v
 with ebind_id  (A : Set) (f : A [⇒] A) (e : expr A) :
+  f ≡ ı → bind f e = e
+with kbind_id  (A : Set) (f : A [⇒] A) (e : cont A) :
   f ≡ ı → bind f e = e.
 Proof.
   - auto_bind_id.
     rewrite ebind_id; [reflexivity |].
     apply lift_id, lift_id; assumption.
   - auto_bind_id.
+  - auto_bind_id.
 Qed.
-
-Definition kbind_id  (A : Set) (f : A [⇒] A) (e : ectx A) :
-  f ≡ ı → bind f e = e.
-Proof.
-  rewrite /bind /BindCore_ectx /kbind => H.
-  rewrite <-List.map_id. do 2 f_equal.
-  extensionality x. case : x => // >; rewrite !(ebind_id, vbind_id)//.
-Qed.
-
 
 
 Fixpoint vbind_comp (A B C : Set) (f : B [⇒] C) (g : A [⇒] B) h (v : val A) :
   f ∘ g ≡ h → bind f (bind g v) = bind h v
 with ebind_comp (A B C : Set) (f : B [⇒] C) (g : A [⇒] B) h (e : expr A) :
+  f ∘ g ≡ h → bind f (bind g e) = bind h e
+with kbind_comp (A B C : Set) (f : B [⇒] C) (g : A [⇒] B) h (e : cont A) :
   f ∘ g ≡ h → bind f (bind g e) = bind h e.
 Proof.
   - auto_bind_comp.
@@ -302,15 +246,7 @@ Proof.
     erewrite lift_comp; [reflexivity |].
     erewrite lift_comp; [reflexivity | assumption].
   - auto_bind_comp.
-Qed.
-
-Definition kbind_comp (A B C : Set) (f : B [⇒] C) (g : A [⇒] B) h (e : ectx A) :
-  f ∘ g ≡ h → bind f (bind g e) = bind h e.
-Proof.
-  rewrite /bind/BindCore_ectx/kbind => H.
-  rewrite map_map. do 2 f_equal. extensionality x.
-  case : x => // >; rewrite !(ebind_comp _ _ _ _ _ h,
-                                vbind_comp _ _ _ _ _ h)//.
+  - auto_bind_comp.
 Qed.
 
 
@@ -322,15 +258,10 @@ Qed.
 Proof.
   split; intros; [now apply ebind_id | now apply ebind_comp].
 Qed.
-#[export] Instance Bind_ectx : Bind ectx.
+#[export] Instance Bind_cont : Bind cont.
 Proof.
   split; intros; [now apply kbind_id | now apply kbind_comp].
 Qed.
-
-
-
-(* Definition LamV {S : Set} (e : expr (inc S)) : val S := *)
-(*   RecV (shift e). *)
 
 
 Definition to_val {S} (e : expr S) : option (val S) :=
@@ -352,114 +283,109 @@ Definition nat_op_interp {S} (n : nat_op) (x y : val S) : option (val S) :=
   | _,_ => None
   end.
 
-
-Definition ctx_el_to_expr {X : Set} (K : ectx_el X) (e : expr X) : expr X :=
+Fixpoint fill {X : Set} (K : cont X) (e : expr X) : expr X :=
   match K with
-  (* | OutputK => Output $ e *)
-  | IfK e1 e2 => If e e1 e2
-  | AppLK v => App e (Val v)
-  | AppRK el => App el e
-  | NatOpLK op v => NatOp op e (Val v)
-  | NatOpRK op el => NatOp op el e
-  | ResetK => Reset e
-  end.
-
-Definition fill {X : Set} (K : ectx X) (e : expr X) : expr X :=
-  fold_left (fun e c => ctx_el_to_expr c e) K e.
-
-
-Fixpoint trim_to_first_reset {X : Set} (K : ectx X) (acc : ectx X) : (ectx X * ectx X) :=
-  match K with
-  (* | OutputK :: K => trim_to_first_reset K (OutputK :: acc) *)
-  (* | (IfK e1 e2) :: K => trim_to_first_reset K ((IfK e1 e2) :: acc) *)
-  (* | (AppLK v) :: K => trim_to_first_reset K ((AppLK v) :: acc) *)
-  (* | (AppRK el) :: K => trim_to_first_reset K ((AppRK el) :: acc) *)
-  (* | (NatOpLK op v) :: K => trim_to_first_reset K ((NatOpLK op v) :: acc) *)
-  (* | (NatOpRK op el) :: K => trim_to_first_reset K ((NatOpRK op el) :: acc) *)
-  | (ResetK) :: K => (acc, ResetK :: K)
-  | C :: K => trim_to_first_reset K (C :: acc)
-  | [] => (acc, [])
+  | IfK e1 e2 K => fill K (If e e1 e2)
+  | END => e
+  | AppLK v K => fill K (App e (Val v))
+  | AppRK el K => fill K (App el e)
+  | NatOpLK op v K => fill K (NatOp op e (Val v))
+  | NatOpRK op el K => fill K (NatOp op el e)
   end.
 
 
-
-(* Separate continuation [K] on innermost [reset] *)
-Definition shift_context {X : Set} (K : ectx X) : (ectx X * ectx X) :=
-  let (Ki, Ko) := trim_to_first_reset K [] in
-  (List.rev Ki, Ko).
-
-
-
-Lemma trim_to_first_reset_app {X : Set} (K Ki Ko acc : ectx X) :
-  (Ki, Ko) = trim_to_first_reset K acc ->
-  (List.rev Ki) ++ Ko = (List.rev acc) ++ K.
-Proof.
-  revert Ki Ko acc. induction K; simpl; intros.
-  - by inversion H.
-  - specialize (IHK Ki Ko (a :: acc)) as HI.
-    destruct a; try (specialize (HI H); rewrite HI; simpl;
-                  rewrite -app_assoc; symmetry; apply cons_middle).
-    by inversion H.
-Qed.
+(* Fixpoint trim_to_first_reset {X : Set} (K : ectx X) (acc : ectx X) : (ectx X * ectx X) := *)
+(*   match K with *)
+(*   (* | OutputK :: K => trim_to_first_reset K (OutputK :: acc) *) *)
+(*   (* | (IfK e1 e2) :: K => trim_to_first_reset K ((IfK e1 e2) :: acc) *) *)
+(*   (* | (AppLK v) :: K => trim_to_first_reset K ((AppLK v) :: acc) *) *)
+(*   (* | (AppRK el) :: K => trim_to_first_reset K ((AppRK el) :: acc) *) *)
+(*   (* | (NatOpLK op v) :: K => trim_to_first_reset K ((NatOpLK op v) :: acc) *) *)
+(*   (* | (NatOpRK op el) :: K => trim_to_first_reset K ((NatOpRK op el) :: acc) *) *)
+(*   | (ResetK) :: K => (acc, ResetK :: K) *)
+(*   | C :: K => trim_to_first_reset K (C :: acc) *)
+(*   | [] => (acc, []) *)
+(*   end. *)
 
 
-Lemma shift_context_app {X : Set} (K Ki Ko : ectx X) :
-  (Ki, Ko) = shift_context K -> K = Ki ++ Ko.
-Proof.
-  unfold shift_context. intro.
-  destruct (trim_to_first_reset K ([])) as [Ki' Ko'] eqn:He.
-  inversion H. subst.
-  trans (rev [] ++ K); first auto. symmetry.
-  by apply trim_to_first_reset_app.
-Qed.
+
+(* (* Separate continuation [K] on innermost [reset] *) *)
+(* Definition shift_context {X : Set} (K : ectx X) : (ectx X * ectx X) := *)
+(*   let (Ki, Ko) := trim_to_first_reset K [] in *)
+(*   (List.rev Ki, Ko). *)
 
 
-Lemma trim_reset_no_reset {X : Set} (K Ki Ko acc : ectx X) :
-  (Ki, Ko) = trim_to_first_reset K acc ->
-  ResetK ∉ acc ->
-  ResetK ∉ Ki.
-Proof.
-  elim: K Ko acc Ki; simpl; intros.
-  - congruence.
-  - destruct a; try solve [eapply H; try eapply H0; try (apply not_elem_of_cons; done)].
-    congruence.
-Qed.
+
+(* Lemma trim_to_first_reset_app {X : Set} (K Ki Ko acc : ectx X) : *)
+(*   (Ki, Ko) = trim_to_first_reset K acc -> *)
+(*   (List.rev Ki) ++ Ko = (List.rev acc) ++ K. *)
+(* Proof. *)
+(*   revert Ki Ko acc. induction K; simpl; intros. *)
+(*   - by inversion H. *)
+(*   - specialize (IHK Ki Ko (a :: acc)) as HI. *)
+(*     destruct a; try (specialize (HI H); rewrite HI; simpl; *)
+(*                   rewrite -app_assoc; symmetry; apply cons_middle). *)
+(*     by inversion H. *)
+(* Qed. *)
 
 
-Lemma shift_context_no_reset {X : Set} (K Ki Ko : ectx X) :
-  (Ki, Ko) = shift_context K -> ResetK ∉ Ki.
-Proof.
-  rewrite /shift_context//. destruct (trim_to_first_reset K []) eqn:Heq. symmetry in Heq.
-  intros. eapply trim_reset_no_reset in Heq; last apply not_elem_of_nil.
-  rewrite rev_alt in H. inversion H. subst. by rewrite elem_of_reverse.
-Qed.
+(* Lemma shift_context_app {X : Set} (K Ki Ko : ectx X) : *)
+(*   (Ki, Ko) = shift_context K -> K = Ki ++ Ko. *)
+(* Proof. *)
+(*   unfold shift_context. intro. *)
+(*   destruct (trim_to_first_reset K ([])) as [Ki' Ko'] eqn:He. *)
+(*   inversion H. subst. *)
+(*   trans (rev [] ++ K); first auto. symmetry. *)
+(*   by apply trim_to_first_reset_app. *)
+(* Qed. *)
 
 
-Lemma no_reset_trim_ident {X : Set} (K acc : ectx X) :
-  ResetK ∉ K -> ResetK ∉ acc ->
-  ((List.rev K) ++ acc, []) = trim_to_first_reset K acc.
-  Proof.
-    elim: K acc; intros; simpl; eauto.
-    apply not_elem_of_cons in H0 as [Hh Ht].
-    destruct a; try contradiction;
-      rewrite -app_assoc; simpl; apply H; eauto; by apply not_elem_of_cons.
-  Qed.
+(* Lemma trim_reset_no_reset {X : Set} (K Ki Ko acc : ectx X) : *)
+(*   (Ki, Ko) = trim_to_first_reset K acc -> *)
+(*   ResetK ∉ acc -> *)
+(*   ResetK ∉ Ki. *)
+(* Proof. *)
+(*   elim: K Ko acc Ki; simpl; intros. *)
+(*   - congruence. *)
+(*   - destruct a; try solve [eapply H; try eapply H0; try (apply not_elem_of_cons; done)]. *)
+(*     congruence. *)
+(* Qed. *)
 
 
-Lemma no_reset_shift_context_ident {X : Set} (K : ectx X) :
-  ResetK ∉ K -> (K, []) = shift_context K.
-Proof.
-  unfold shift_context. intros. rewrite -no_reset_trim_ident;
-    last apply not_elem_of_nil; last done.
-  by rewrite app_nil_r rev_involutive.
-Qed.
+(* Lemma shift_context_no_reset {X : Set} (K Ki Ko : ectx X) : *)
+(*   (Ki, Ko) = shift_context K -> ResetK ∉ Ki. *)
+(* Proof. *)
+(*   rewrite /shift_context//. destruct (trim_to_first_reset K []) eqn:Heq. symmetry in Heq. *)
+(*   intros. eapply trim_reset_no_reset in Heq; last apply not_elem_of_nil. *)
+(*   rewrite rev_alt in H. inversion H. subst. by rewrite elem_of_reverse. *)
+(* Qed. *)
+
+
+(* Lemma no_reset_trim_ident {X : Set} (K acc : ectx X) : *)
+(*   ResetK ∉ K -> ResetK ∉ acc -> *)
+(*   ((List.rev K) ++ acc, []) = trim_to_first_reset K acc. *)
+(*   Proof. *)
+(*     elim: K acc; intros; simpl; eauto. *)
+(*     apply not_elem_of_cons in H0 as [Hh Ht]. *)
+(*     destruct a; try contradiction; *)
+(*       rewrite -app_assoc; simpl; apply H; eauto; by apply not_elem_of_cons. *)
+(*   Qed. *)
+
+
+(* Lemma no_reset_shift_context_ident {X : Set} (K : ectx X) : *)
+(*   ResetK ∉ K -> (K, []) = shift_context K. *)
+(* Proof. *)
+(*   unfold shift_context. intros. rewrite -no_reset_trim_ident; *)
+(*     last apply not_elem_of_nil; last done. *)
+(*   by rewrite app_nil_r rev_involutive. *)
+(* Qed. *)
 
 
 (* Only if no reset in K *)
-Definition cont_to_rec {X : Set} (K : ectx X) : (val X) :=
-  ContV (fill (shift K) (Var VZ)).
+(* Definition cont_to_rec {X : Set} (K : ectx X) : (val X) := *)
+(*   ContV (fill (shift K) (Var VZ)). *)
 
-Example test1 : val (inc ∅) := (cont_to_rec [(NatOpLK Add (LitV 3)); AppRK (Var VZ)]).
+(* Example test1 : val (inc ∅) := (cont_to_rec [(NatOpLK Add (LitV 3)); AppRK (Var VZ)]). *)
 
 (* Lemma fill_emap {X Y : Set} (f : X [→] Y) (K : ectx X) (e : expr X) *)
 (*   : fmap f (fill K e) = fill (fmap f K) (fmap f e). *)
@@ -491,100 +417,109 @@ Example test1 : val (inc ∅) := (cont_to_rec [(NatOpLK Add (LitV 3)); AppRK (Va
 
 (** [head_step e σ K e' σ' K' Ko (n, m)] : step from [(e, σ, K)] to [(e', σ', K')]
     under outer context [Ko] in [n] ticks with [m] effects encountered *)
-Variant head_step {S} : expr S -> ectx S ->
-                        expr S -> ectx S ->
-                        ectx S ->
-                        nat * nat → Prop :=
-  | BetaS e1 v2 K Ko :
-    head_step (App (Val $ RecV e1) (Val v2)) K
-      (subst (Inc := inc) ((subst (F := expr) (Inc := inc) e1)
-                             (Val (shift (Inc := inc) v2)))
-         (Val (RecV e1))) K Ko (1,0)
-  | BetaContS e1 v2 K Ko :
-    head_step (App (Val $ ContV e1) (Val v2)) K
-      (subst  (Inc := inc) e1 (Val  v2))
-      K Ko (2,0)
-  (* | InputS n σ' K Ko : *)
-  (*   update_input = (n, σ') → *)
-  (*   head_step Input K (Val (LitV n)) σ' K Ko (1, 1) *)
-  (* | OutputS n σ' K Ko : *)
-  (*   update_output n = σ' → *)
-  (*   head_step (Output (Val (LitV n))) K (Val (LitV 0)) σ' K Ko (1, 1) *)
-  | NatOpS op v1 v2 v3 K Ko :
-    nat_op_interp op v1 v2 = Some v3 →
-    head_step (NatOp op (Val v1) (Val v2)) K
-      (Val v3) K Ko (0, 0)
-  | IfTrueS n e1 e2 K Ko :
-    n > 0 →
-    head_step (If (Val (LitV n)) e1 e2) K
-      e1 K Ko (0, 0)
-  | IfFalseS n e1 e2 K Ko :
-    n = 0 →
-    head_step (If (Val (LitV n)) e1 e2) K
-      e2 K Ko (0, 0)
+(* Variant head_step {S} : expr S -> ectx S -> *)
+(*                         expr S -> ectx S -> *)
+(*                         ectx S -> *)
+(*                         nat * nat → Prop := *)
+(*   | BetaS e1 v2 K Ko : *)
+(*     head_step (App (Val $ RecV e1) (Val v2)) K *)
+(*       (subst (Inc := inc) ((subst (F := expr) (Inc := inc) e1) *)
+(*                              (Val (shift (Inc := inc) v2))) *)
+(*          (Val (RecV e1))) K Ko (1,0) *)
+(*   | BetaContS e1 v2 K Ko : *)
+(*     head_step (App (Val $ ContV e1) (Val v2)) K *)
+(*       (subst  (Inc := inc) e1 (Val  v2)) *)
+(*       K Ko (2,0) *)
+(*   (* | InputS n σ' K Ko : *) *)
+(*   (*   update_input = (n, σ') → *) *)
+(*   (*   head_step Input K (Val (LitV n)) σ' K Ko (1, 1) *) *)
+(*   (* | OutputS n σ' K Ko : *) *)
+(*   (*   update_output n = σ' → *) *)
+(*   (*   head_step (Output (Val (LitV n))) K (Val (LitV 0)) σ' K Ko (1, 1) *) *)
+(*   | NatOpS op v1 v2 v3 K Ko : *)
+(*     nat_op_interp op v1 v2 = Some v3 → *)
+(*     head_step (NatOp op (Val v1) (Val v2)) K *)
+(*       (Val v3) K Ko (0, 0) *)
+(*   | IfTrueS n e1 e2 K Ko : *)
+(*     n > 0 → *)
+(*     head_step (If (Val (LitV n)) e1 e2) K *)
+(*       e1 K Ko (0, 0) *)
+(*   | IfFalseS n e1 e2 K Ko : *)
+(*     n = 0 → *)
+(*     head_step (If (Val (LitV n)) e1 e2) K *)
+(*       e2 K Ko (0, 0) *)
 
-  | ShiftS (e : expr (inc (inc S))) K Ko f :
-    ResetK ∉ K ->
-    f = cont_to_rec (ResetK::K) ->
-    head_step (Shift (Val $ RecV e)) K
-      (subst (Inc := inc) ((subst (F := expr) (Inc := inc) e)
-                             (Val (shift (Inc := inc) f)))
-         (Val $ RecV e)) [] Ko (1, 1)
+(*   | ShiftS (e : expr (inc (inc S))) K Ko f : *)
+(*     ResetK ∉ K -> *)
+(*     f = cont_to_rec (ResetK::K) -> *)
+(*     head_step (Shift (Val $ RecV e)) K *)
+(*       (subst (Inc := inc) ((subst (F := expr) (Inc := inc) e) *)
+(*                              (Val (shift (Inc := inc) f))) *)
+(*          (Val $ RecV e)) [] Ko (1, 1) *)
 
-  | ResetS v K Ko :
-    head_step (Reset (Val v)) K (Val v) K Ko (1, 1).
+(*   | ResetS v K Ko : *)
+(*     head_step (Reset (Val v)) K (Val v) K Ko (1, 1). *)
 
 
-  (* | ValueS v σ K C: *)
-  (*   head_step (Val v) σ (C::K) (ctx_el_to_expr C (Val v)) σ K (0, 0) *)
+(*   (* | ValueS v σ K C: *) *)
+(*   (*   head_step (Val v) σ (C::K) (ctx_el_to_expr C (Val v)) σ K (0, 0) *) *)
 
-  (* | ResetShiftS e σ K E: *)
-  (*   head_step *)
-  (*     (Reset (fill E (Shift e))) σ *)
-  (*     (Reset (subst (Inc := inc) e (Val $ ContV $ ResetK E))) σ K (1,0). *)
+(*   (* | ResetShiftS e σ K E: *) *)
+(*   (*   head_step *) *)
+(*   (*     (Reset (fill E (Shift e))) σ *) *)
+(*   (*     (Reset (subst (Inc := inc) e (Val $ ContV $ ResetK E))) σ K (1,0). *) *)
 
-Lemma head_step_io_01 {S} (e1 e2 : expr S) K K' Ko n m :
-  head_step e1 K e2 K' Ko (n,m) → m = 0 ∨ m = 1.
-Proof.  inversion 1; eauto. Qed.
-(* Lemma head_step_unfold_01 {S} (e1 e2 : expr S) σ1 σ2 K K' n m : *)
-(*   head_step e1 σ1 K e2 σ2 K' (n,m) → n = 0 ∨ n = 1. *)
+(* Lemma head_step_io_01 {S} (e1 e2 : expr S) K K' Ko n m : *)
+(*   head_step e1 K e2 K' Ko (n,m) → m = 0 ∨ m = 1. *)
 (* Proof.  inversion 1; eauto. Qed. *)
-(* Lemma head_step_no_io {S} (e1 e2 : expr S) σ1 σ2 K K' Ko n : *)
-(*   head_step e1 σ1 K e2 σ2 K' Ko (n,0) → σ1 = σ2. *)
-(* Proof.  inversion 1; eauto. Qed. *)
+(* (* Lemma head_step_unfold_01 {S} (e1 e2 : expr S) σ1 σ2 K K' n m : *) *)
+(* (*   head_step e1 σ1 K e2 σ2 K' (n,m) → n = 0 ∨ n = 1. *) *)
+(* (* Proof.  inversion 1; eauto. Qed. *) *)
+(* (* Lemma head_step_no_io {S} (e1 e2 : expr S) σ1 σ2 K K' Ko n : *) *)
+(* (*   head_step e1 σ1 K e2 σ2 K' Ko (n,0) → σ1 = σ2. *) *)
+(* (* Proof.  inversion 1; eauto. Qed. *) *)
 
-(** Carbonara from heap lang *)
+(* (** Carbonara from heap lang *) *)
 
-Global Instance ctx_el_to_expr_inj {S} (C : ectx_el S) : Inj (=) (=) (ctx_el_to_expr C).
-Proof. case: C => [] >; simpl in*; congruence. Qed.
+(* Global Instance ctx_el_to_expr_inj {S} (C : ectx_el S) : Inj (=) (=) (ctx_el_to_expr C). *)
+(* Proof. case: C => [] >; simpl in*; congruence. Qed. *)
 
-Global Instance fill_inj {S} (Ki : ectx S) : Inj (=) (=) (fill Ki).
+Global Instance fill_inj {S} (Ki : cont S) : Inj (=) (=) (fill Ki).
 Proof. induction Ki; intros ???; simplify_eq/=; auto with f_equal. Qed.
 
-Lemma ctx_el_to_expr_val {S} C (e : expr S) :
-  is_Some (to_val (ctx_el_to_expr C e)) → is_Some (to_val e).
-Proof. case : C => [] > H; simpl in H; try by apply is_Some_None in H. Qed.
+(* Lemma ctx_el_to_expr_val {S} C (e : expr S) : *)
+(*   is_Some (to_val (ctx_el_to_expr C e)) → is_Some (to_val e). *)
+(* Proof. case : C => [] > H; simpl in H; try by apply is_Some_None in H. Qed. *)
 
 Lemma fill_val {S} Ki (e : expr S) :
   is_Some (to_val (fill Ki e)) → is_Some (to_val e).
-Proof. elim: Ki e; simpl in *; first done. intros.
-       apply (ctx_el_to_expr_val a e). apply H. apply H0.
+Proof.
+  elim: Ki e; simpl in *; intros; first done;
+    apply H in H0; simpl in H0; contradiction (is_Some_None H0).
 Qed.
 
-(* CHECK *)
-Lemma val_head_stuck {S} (e1 : expr S) e2 K K' Ko m :
-  head_step e1 K e2 K' Ko m → to_val e1 = None.
-Proof. destruct 1; naive_solver. Qed.
+(* (* CHECK *) *)
+(* Lemma val_head_stuck {S} (e1 : expr S) e2 K K' Ko m : *)
+(*   head_step e1 K e2 K' Ko m → to_val e1 = None. *)
+(* Proof. destruct 1; naive_solver. Qed. *)
 
 
 (* K1 ∘ K2 *)
-Definition ectx_compose {S} (K1 K2 : ectx S) : ectx S :=
-  K2 ++ K1.
+Fixpoint cont_compose {S} (K1 K2 : cont S) : cont S :=
+  match K2 with
+  | END => K1
+  | IfK e1 e2 K => IfK e1 e2 (cont_compose K1 K)
+  | AppLK v K => AppLK v (cont_compose K1 K)
+  | AppRK e K => AppRK e (cont_compose K1 K)
+  | NatOpLK op v K => NatOpLK op v (cont_compose K1 K)
+  | NatOpRK op e K => NatOpRK op e (cont_compose K1 K)
+  end.
 
-Lemma fill_app {S} (K1 K2 : ectx S) e : fill (ectx_compose K1 K2) e = fill K1 (fill K2 e).
+
+Lemma fill_comp {S} (K1 K2 : cont S) e : fill (cont_compose K1 K2) e = fill K1 (fill K2 e).
 Proof.
-  elim: K2 K1 e =>>; eauto.
-  intros H K1 e. simpl. by rewrite H.
+  elim: K2 K1 e =>>; eauto;
+  intros H K1 e; simpl; by rewrite H.
 Qed.
 
 
@@ -595,94 +530,90 @@ Proof.
 Qed.
 
 
-Lemma fill_comp {S} K1 K2 (e : expr S) : fill K2 (fill K1 e) = fill (ectx_compose K2 K1) e.
-Proof. by rewrite fill_app. Qed.
-
-
 (* FIXME maybe *)
-Inductive prim_step {S} : ∀ (e1 : expr S) 
-          (e2 : expr S) (nm : nat * nat), Prop :=
-(* | Ectx_step e1 σ1 e2 σ2 nm (K1 K2 : ectx S) e1' e2' : *)
-(*   e1 = fill K1 e1' -> *)
-(*   e2 = fill K2 e2' -> *)
-(*   ResetK ∉ K1 -> *)
-(*   head_step e1' σ1 K1 e2' σ2 K2 nm -> *)
-(*   prim_step e1 σ1 e2 σ2 nm *)
-| Shift_step e1 K Ki Ko e2 Ki' nm :
-  (Ki, Ko) = shift_context K ->
-  head_step e1 Ki e2 Ki' Ko nm ->
-  prim_step (fill K e1) (fill (Ki' ++ Ko) e2) nm.
-(* CHECK *)
+(* Inductive prim_step {S} : ∀ (e1 : expr S)  *)
+(*           (e2 : expr S) (nm : nat * nat), Prop := *)
+(* (* | Ectx_step e1 σ1 e2 σ2 nm (K1 K2 : ectx S) e1' e2' : *) *)
+(* (*   e1 = fill K1 e1' -> *) *)
+(* (*   e2 = fill K2 e2' -> *) *)
+(* (*   ResetK ∉ K1 -> *) *)
+(* (*   head_step e1' σ1 K1 e2' σ2 K2 nm -> *) *)
+(* (*   prim_step e1 σ1 e2 σ2 nm *) *)
+(* | Shift_step e1 K Ki Ko e2 Ki' nm : *)
+(*   (Ki, Ko) = shift_context K -> *)
+(*   head_step e1 Ki e2 Ki' Ko nm -> *)
+(*   prim_step (fill K e1) (fill (Ki' ++ Ko) e2) nm. *)
+(* (* CHECK *) *)
 
-(* Lemma prim_step_pure {S} (e1 e2 : expr S) σ1 σ2 n : *)
-(*   prim_step e1 σ1 e2 σ2 (n,0) → σ1 = σ2. *)
+(* (* Lemma prim_step_pure {S} (e1 e2 : expr S) σ1 σ2 n : *) *)
+(* (*   prim_step e1 σ1 e2 σ2 (n,0) → σ1 = σ2. *) *)
+(* (* Proof. *) *)
+(* (*   inversion 1; simplify_eq/=. by inversion H1. *) *)
+(* (* Qed. *) *)
+
+(* Inductive prim_steps {S} : expr S → expr S → nat * nat → Prop := *)
+(* | prim_steps_zero e : *)
+(*   prim_steps e e (0, 0) *)
+(* | prim_steps_abit e1 e2 e3 n1 m1 n2 m2 : *)
+(*   prim_step e1 e2 (n1, m1) → *)
+(*   prim_steps e2 e3 (n2, m2) → *)
+(*   prim_steps e1 e3 (plus n1 n2, plus m1 m2) *)
+(* . *)
+
+(* Lemma Ectx_step' {S} (K1 K2 : ectx S) e1 e2 efs : *)
+(*   head_step e1 K1 e2 K2 [] efs → *)
+(*   ResetK ∉ K1 -> *)
+(*   prim_step (fill K1 e1) (fill K2 e2) efs. *)
 (* Proof. *)
-(*   inversion 1; simplify_eq/=. by inversion H1. *)
+(*   intros. rewrite -(app_nil_r K2). *)
+(*   econstructor; eauto. by apply no_reset_shift_context_ident. *)
 (* Qed. *)
 
-Inductive prim_steps {S} : expr S → expr S → nat * nat → Prop :=
-| prim_steps_zero e :
-  prim_steps e e (0, 0)
-| prim_steps_abit e1 e2 e3 n1 m1 n2 m2 :
-  prim_step e1 e2 (n1, m1) →
-  prim_steps e2 e3 (n2, m2) →
-  prim_steps e1 e3 (plus n1 n2, plus m1 m2)
-.
+(* Lemma prim_steps_app {S} nm1 nm2 (e1 e2 e3 : expr S) : *)
+(*   prim_steps e1 e2 nm1 → prim_steps e2 e3 nm2 → *)
+(*   prim_steps e1 e3 (plus nm1.1 nm2.1, plus nm1.2 nm2.2). *)
+(* Proof. *)
+(*   intros Hst. revert nm2. *)
+(*   induction Hst; intros [n' m']; simplify_eq/=; first done. *)
+(*   rewrite -!Nat.add_assoc. intros Hsts. *)
+(*   econstructor; eauto. *)
+(*   by apply (IHHst (n',m')). *)
+(* Qed. *)
 
-Lemma Ectx_step' {S} (K1 K2 : ectx S) e1 e2 efs :
-  head_step e1 K1 e2 K2 [] efs →
-  ResetK ∉ K1 ->
-  prim_step (fill K1 e1) (fill K2 e2) efs.
-Proof.
-  intros. rewrite -(app_nil_r K2).
-  econstructor; eauto. by apply no_reset_shift_context_ident.
-Qed.
+(* Lemma prim_step_steps {S} nm (e1 e2 : expr S) : *)
+(*   prim_step e1 e2 nm → prim_steps e1 e2 nm. *)
+(* Proof. *)
+(*   destruct nm as [n m]. intro Hs. *)
+(*   rewrite -(Nat.add_0_r n). *)
+(*   rewrite -(Nat.add_0_r m). *)
+(*   econstructor; eauto. *)
+(*   by constructor. *)
+(* Qed. *)
 
-Lemma prim_steps_app {S} nm1 nm2 (e1 e2 e3 : expr S) :
-  prim_steps e1 e2 nm1 → prim_steps e2 e3 nm2 →
-  prim_steps e1 e3 (plus nm1.1 nm2.1, plus nm1.2 nm2.2).
-Proof.
-  intros Hst. revert nm2.
-  induction Hst; intros [n' m']; simplify_eq/=; first done.
-  rewrite -!Nat.add_assoc. intros Hsts.
-  econstructor; eauto.
-  by apply (IHHst (n',m')).
-Qed.
+(* Lemma prim_step_steps_steps {S} (e1 e2 e3 : expr S) nm1 nm2 nm3 : *)
+(*   nm3 = (plus nm1.1 nm2.1, plus nm1.2 nm2.2) -> *)
+(*   prim_step e1 e2 nm1 → prim_steps e2 e3 nm2 -> prim_steps e1 e3 nm3. *)
+(* Proof. *)
+(*   intros -> H G. *)
+(*   eapply prim_steps_app; last apply G. *)
+(*   apply prim_step_steps, H. *)
+(* Qed. *)
 
-Lemma prim_step_steps {S} nm (e1 e2 : expr S) :
-  prim_step e1 e2 nm → prim_steps e1 e2 nm.
-Proof.
-  destruct nm as [n m]. intro Hs.
-  rewrite -(Nat.add_0_r n).
-  rewrite -(Nat.add_0_r m).
-  econstructor; eauto.
-  by constructor.
-Qed.
-
-Lemma prim_step_steps_steps {S} (e1 e2 e3 : expr S) nm1 nm2 nm3 :
-  nm3 = (plus nm1.1 nm2.1, plus nm1.2 nm2.2) ->
-  prim_step e1 e2 nm1 → prim_steps e2 e3 nm2 -> prim_steps e1 e3 nm3.
-Proof.
-  intros -> H G.
-  eapply prim_steps_app; last apply G.
-  apply prim_step_steps, H.
-Qed.
-
-Lemma head_step_prim_step {S} (e1 e2 : expr S) nm :
-  head_step e1 [] e2 [] [] nm -> prim_step e1 e2 nm.
-Proof.
-  move => H; apply Ectx_step' in H => //=. apply not_elem_of_nil.
-Qed.
+(* Lemma head_step_prim_step {S} (e1 e2 : expr S) nm : *)
+(*   head_step e1 [] e2 [] [] nm -> prim_step e1 e2 nm. *)
+(* Proof. *)
+(*   move => H; apply Ectx_step' in H => //=. apply not_elem_of_nil. *)
+(* Qed. *)
 
 
 (*** Abstract Machine semantics *)
 
-Definition Mectx {S} := list $ ectx S.
+Definition Mcont {S} := list $ cont S.
 
 Variant config {S} : Type :=
-  | Ceval : expr S -> ectx S -> @Mectx S -> config
-  | Ccont : ectx S -> val S -> @Mectx S -> config
-  | Cmcont : @Mectx S -> val S -> config
+  | Ceval : expr S -> cont S -> @Mcont S -> config
+  | Ccont : cont S -> val S -> @Mcont S -> config
+  | Cmcont : @Mcont S -> val S -> config
   | Cexpr : expr S -> config
   | Cret : val S -> config.
 
@@ -693,69 +624,59 @@ Variant Cred {S : Set} : config -> config -> (nat * nat) -> Prop :=
 
   (* init *)
   | Ceval_init : forall (e : expr S),
-      Cexpr e ===> Ceval e [] [] / (0,0)
+      Cexpr e ===> Ceval e END [] / (0,0)
 
   (* eval *)
   | Ceval_val : forall v k mk,
       Ceval (Val v) k mk ===> Ccont k v mk / (0,0)
 
   | Ceval_app : forall e0 e1 k mk,
-      Ceval (App e0 e1) k mk ===> Ceval e1 (AppRK e0 :: k) mk / (0,0)
+      Ceval (App e0 e1) k mk ===> Ceval e1 (AppRK e0 k) mk / (0,0)
 
   | Ceval_natop : forall op e0 e1 k mk,
-      Ceval (NatOp op e0 e1) k mk ===> Ceval e1 (NatOpRK op e0 :: k) mk / (0,0)
+      Ceval (NatOp op e0 e1) k mk ===> Ceval e1 (NatOpRK op e0 k) mk / (0,0)
 
   | Ceval_if : forall eb et ef k mk,
-      Ceval (If eb et ef) k mk ===> Ceval eb (IfK et ef :: k) mk / (0,0)
+      Ceval (If eb et ef) k mk ===> Ceval eb (IfK et ef k) mk / (0,0)
 
   | Ceval_reset : forall e k mk,
-      Ceval (Reset e) k mk ===> Ceval e [] (k :: mk) / (1, 1)
+      Ceval (Reset e) k mk ===> Ceval e END (k :: mk) / (1, 1)
 
-  | Ceval_shift : forall (e : expr $ inc $ inc S) k f mk,
-      f = cont_to_rec (k) ->    (* CHECK: should we add a reset to ctx ? don't think so *)
-      Ceval (Shift $ Val $ RecV e) k mk ===>
-        Ceval (subst (Inc := inc)
-                 (subst (F := expr) (Inc := inc)
-                    e (Val (shift (Inc:=inc) f)))
-                 (Val (RecV e))) [] mk / (1, 1)
+  | Ceval_shift : forall (e : expr $ inc S) k mk,
+      Ceval (Shift e) k mk ===>
+        Ceval (subst (Inc := inc) e (Val $ ContV k))
+        END mk / (1, 1)
 
   (* cont *)
-  | Ccont_hole : forall v mk,
-      Ccont [] v mk ===> Cmcont mk v / (0,0)
+  | Ccont_end : forall v mk,
+      Ccont END v mk ===> Cmcont mk v / (0,0)
 
   | Ccont_appr : forall e v k mk,
-      Ccont (AppRK e :: k) v mk ===> Ceval e (AppLK v :: k) mk / (0, 0)
+      Ccont (AppRK e k) v mk ===> Ceval e (AppLK v k) mk / (0, 0)
 
   | Ccont_appl : forall e v k mk,
-      Ccont (AppLK v :: k) (RecV e) mk ===>
+      Ccont (AppLK v k) (RecV e) mk ===>
         Ceval (subst (Inc := inc)
                  (subst (F := expr) (Inc := inc) e
                     (Val (shift (Inc := inc) v)))
                  (Val (RecV e))) k mk / (1, 0)
 
-  | Ccont_cont : forall e v k mk,
-      Ccont (AppLK v :: k) (ContV e) mk ===>
-        Ceval (subst (Inc := inc) e (Val v)) [] (k :: mk) / (2, 0)
+  | Ccont_cont : forall v k k' mk,
+      Ccont (AppLK v k) (ContV k') mk ===>
+        Ccont k' v (k :: mk) / (2, 0)
 
-  | Ccont_ift : forall et ef n k mk,
-      n > 0 ->
-      Ccont (IfK et ef :: k) (LitV n) mk ===>
-        Ceval et k mk / (0, 0)
-
-  | Ccont_iff : forall et ef n k mk,
-      n = 0 ->
-      Ccont (IfK et ef :: k) (LitV n) mk ===>
-        Ceval ef k mk / (0, 0)
+  | Ccont_if : forall et ef n k mk,
+      Ccont (IfK et ef k) (LitV n) mk ===>
+        Ceval (if (n =? 0) then ef else et) k mk / (0, 0)
 
   | Ccont_natopr : forall op e v k mk,
-      Ccont (NatOpRK op e :: k) v mk ===>
-        Ceval e (NatOpLK op v :: k) mk / (0, 0)
+      Ccont (NatOpRK op e k) v mk ===>
+        Ceval e (NatOpLK op v k) mk / (0, 0)
 
   | Ccont_natopl : forall op v0 v1 v2 k mk,
       nat_op_interp op v0 v1 = Some v2 ->
-      Ccont (NatOpLK op v1 :: k) v0 mk ===>
+      Ccont (NatOpLK op v1 k) v0 mk ===>
         Ceval (Val v2) k mk / (0,0)
-
 
   (* meta-cont *)
   | Cmcont_cont : forall k mk v,
@@ -766,12 +687,12 @@ Variant Cred {S : Set} : config -> config -> (nat * nat) -> Prop :=
 
 where "c ===> c' / nm" := (Cred c c' nm).
 
-Arguments Mectx S%bind : clear implicits.
+Arguments Mcont S%bind : clear implicits.
 Arguments config S%bind : clear implicits.
 
 (** ** On configs & meta-contexts *)
 
-Definition meta_fill {S} (mk : Mectx S) e :=
+Definition meta_fill {S} (mk : Mcont S) e :=
   fold_left (λ e k, fill k e) mk e.
 
 
